Remove predicative invariants.

pulse/lib/core/PulseCore.BaseHeapSig.fsti
@@ -3,11 +3,91 @@ open PulseCore.HeapSig
 open FStar.Ghost
 open FStar.PCM
 module H = PulseCore.Heap
-val base_heap : heap_sig u#a
-val join_empty_inverse (m0 m1:base_heap.mem)
-: Lemma 
-    (requires base_heap.sep.disjoint m0 m1 /\ base_heap.sep.join m0 m1 == base_heap.sep.empty)
-    (ensures m0 == base_heap.sep.empty /\ m1 == base_heap.sep.empty)
+module H2 = PulseCore.Heap2
+
+type mem : Type u#(a + 1) = H2.heap u#a
+
+let empty_mem : mem u#a = H2.empty_heap
+
+let disjoint_mem (m0 m1: mem) : prop = H2.disjoint m0 m1
+
+let join_mem (m0:mem) (m1:mem { disjoint_mem m0 m1 }) : mem = H2.join m0 m1
+
+let sep : separable (mem u#a) = {
+    empty = empty_mem;
+    disjoint = disjoint_mem;
+    join = join_mem;
+    disjoint_sym = (fun m1 m2 -> H2.disjoint_sym m1 m2);
+    join_commutative = (fun h0 h1 -> H2.join_commutative h0 h1); 
+    disjoint_join = (fun m1 m2 m3 -> H2.disjoint_join m1 m2 m3);
+    join_associative = (fun h0 h1 h2 -> H2.join_associative h0 h1 h2);
+    join_empty = (fun m -> H2.join_empty m);
+}
+
+let full_mem_pred m = H2.full_heap_pred m
+
+let is_ghost_action m0 m1 : prop =
+  H2.concrete m0 == H2.concrete m1
+
+let slprop = H2.slprop
+
+val interp (p:slprop u#a) : affine_mem_prop u#(a+1) sep
+
+val as_slprop (p:affine_mem_prop sep) : q:slprop{forall h. interp q h <==> p h}
+
+let emp : slprop = H2.emp
+val pure (p:prop) : slprop
+
+let star (p1:slprop) (p2:slprop) : slprop =
+  H2.star p1 p2
+val star_equiv (p q:slprop u#a) (m:mem u#a)
+: Lemma (
+    interp (p `star` q) m <==> 
+        (exists m0 m1. 
+          sep.disjoint m0 m1 /\
+          m == sep.join m0 m1 /\
+          interp p m0 /\
+          interp q m1)
+  )
+
+val slprop_extensionality (p q:slprop)
+: Lemma ((forall c. interp p c <==> interp q c) ==> p == q)
+
+val interp_as (p:affine_mem_prop sep)
+: Lemma (forall c. interp (as_slprop p) c == p c)
+
+val emp_unit (p:slprop) : Lemma (p == (p `star` emp))
+
+let update_ghost (m0:mem u#a) (m1:erased (mem u#a) { is_ghost_action m0 m1 })
+: m:mem u#a { m == reveal m1 }
+= H2.upd_ghost_heap m0 m1
+
+val pure_true_emp () : Lemma (pure True == emp)
+val intro_emp (h:mem) : Lemma (interp emp h)
+val pure_interp (p:prop) (c:mem) : Lemma (interp (pure p) c == p)
+let base_heap : heap_sig u#a =
+  {
+    mem;
+    sep;
+    full_mem_pred;
+    is_ghost_action;
+    is_ghost_action_preorder= (fun _ -> ());
+    update_ghost;
+    slprop;
+    interp;
+    as_slprop;
+    interp_as;
+    slprop_extensionality;
+    non_info_slprop = (fun x -> reveal x);
+    emp;
+    pure;
+    star;
+    intro_emp;
+    pure_interp;
+    pure_true_emp;
+    emp_unit;
+    star_equiv;
+}
 
 val core_ghost_ref_is_null (c:core_ghost_ref) : GTot bool
 let non_null_core_ghost_ref = r:core_ghost_ref { not (core_ghost_ref_is_null r) }
@@ -30,134 +110,17 @@ val empty_mem_props ()
     free_above_ghost_ctr base_heap.sep.empty /\
     ghost_ctr base_heap.sep.empty == 0
   )
-val mem_invariant_interp (ex:inames base_heap) (h0:base_heap.mem) (h1:base_heap.mem)
-: Lemma (base_heap.interp (base_heap.mem_invariant ex h0) h1 ==>
-         free_above_ghost_ctr h0)
-val inames_ok_trivial (ex:inames base_heap) (h:base_heap.mem)
-: Lemma (inames_ok ex h)
-
-val bump_ghost_ctr (m0:base_heap.mem) (x:erased nat)
-: m1:base_heap.mem {
-    (exists m'. m1 == base_heap.sep.join m0 m') /\
-    (forall a. select_ghost a m0 == select_ghost a m1) /\
-    // m1 == m0 /\
-    ghost_ctr m1 >= ghost_ctr m0 /\
-    ghost_ctr m1 >= x /\
-    (forall ex c0 c1. base_heap.interp (base_heap.mem_invariant ex m0) c0 ==> base_heap.interp (base_heap.mem_invariant ex m1) c1) /\
-    (forall is. inames_ok is m0 <==> inames_ok is m1) /\
-    base_heap.is_ghost_action m0 m1 /\
-    (base_heap.full_mem_pred m0 ==> base_heap.full_mem_pred m1)
-  }
 
 val pts_to (#a:Type u#a) (#p:pcm a) (r:ref a p) (x:a) : (base_heap u#a).slprop
-val ghost_pts_to (meta:bool) (#a:Type u#a) (#p:pcm a) (r:ghost_ref a p) (x:a) : (base_heap u#a).slprop
-val interp_ghost_pts_to 
-      (i:core_ghost_ref)
-      (#meta:bool)
-      (#a:Type u#a)
-      (#pcm:FStar.PCM.pcm a)
-      (v:a)
-      (h0:(base_heap u#a).mem)
-: Lemma
-  (requires base_heap.interp (ghost_pts_to meta #a #pcm i v) h0)
-  (ensures (
-    not (core_ghost_ref_is_null i) /\ (
-    match select_ghost (core_ghost_ref_as_addr i) h0 with
-    | None -> False
-    | Some c ->
-      let H.Ref meta' a' pcm' v' = c in
-      meta == reveal meta' /\
-      a == a' /\
-      pcm == pcm' /\
-      compatible pcm v v')))
-      
-val ghost_pts_to_compatible_equiv 
-      (#meta:bool)
-      (#a:Type)
-      (#pcm:_)
-      (x:ghost_ref a pcm)
-      (v0:a)
-      (v1:a{composable pcm v0 v1})
-: Lemma ((ghost_pts_to meta x v0 `base_heap.star` ghost_pts_to meta x v1) ==
-         (ghost_pts_to meta x (op pcm v0 v1)))
-
-let heap_cell_evolves (h0 h1:option H.cell)
-: prop
-= match h0, h1 with
-  | None, None -> True
-  | None, Some (H.Ref meta _ _ _) -> reveal meta == false
-  | Some (H.Ref meta a p v), Some (H.Ref meta' a' p' v') ->
-    meta == meta' /\ (reveal meta ==> a==a' /\ p==p' /\ v==v')
-  | _, _ -> False
-
-let heaps_preserve_inames (m0 m1:base_heap.mem) =
-  ghost_ctr m0 <= ghost_ctr m1 /\
-  (forall (addr:nat).
-    heap_cell_evolves (select_ghost addr m0) (select_ghost addr m1))
-
-let preserves_inames 
-    (#a:Type u#a)
-    (#mg:bool)
-    (#pre:base_heap.slprop)
-    (#post:a -> GTot (base_heap.slprop))
-    (#ex:inames base_heap)
-    (action:_action_except (base_heap u#h) a mg ex pre post)
-= forall (m0:full_mem base_heap) frame. 
-    interpret (pre `base_heap.star` frame `base_heap.star` base_heap.mem_invariant ex m0) m0 /\
-    inames_ok ex m0
-    ==> ( 
-    let x, m1 = action frame m0 in
-    heaps_preserve_inames m0 m1
-    )
-
-let single_ghost_allocation
-        (meta:bool)
-        (#a:Type)
-        (#pcm:pcm a)
-        (x:a{pcm.refine x})
-        (r:ghost_ref a pcm)
-        (h h1:base_heap.mem)
-= (forall (a:nat).
-    a <> ghost_ctr h ==>
-    select_ghost a h == select_ghost a h1) /\
-  ghost_ctr h1 == ghost_ctr h + 1 /\
-  select_ghost (ghost_ctr h) h1 == Some (H.Ref meta a pcm x) /\
-  addr_as_core_ghost_ref (ghost_ctr h) == r /\
-  free_above_ghost_ctr h /\
-  free_above_ghost_ctr h1
+val ghost_pts_to (#a:Type u#a) (#p:pcm a) (r:ghost_ref a p) (x:a) : (base_heap u#a).slprop
 
 val ghost_extend
-    (meta:erased bool)
-    (#ex:inames base_heap)
-    (#a:Type u#a)
+    (#a:Type)
     (#pcm:pcm a)
     (x:erased a{pcm.refine x})
-: act:ghost_action_except base_heap (ghost_ref a pcm) ex    
-        base_heap.emp 
-        (fun r -> ghost_pts_to meta r x) {
-            reveal meta == false ==> preserves_inames act
-        }
-
-
-  
-val ghost_extend_spec
-      (#meta:bool)
-      (#ex:inames base_heap)
-      (#a:Type u#a) #pcm (x:a { pcm.refine x })
-      (frame:base_heap.slprop)
-      (h:full_mem base_heap { 
-        inames_ok ex h /\
-        interpret (base_heap.emp `base_heap.star`
-                   frame `base_heap.star`
-                   base_heap.mem_invariant ex h) h })      
-: Lemma (
-      let (r, h1) = ghost_extend meta #ex #a #pcm x frame h in
-      single_ghost_allocation meta #a #pcm x r h h1
-)
+: ghost_action_except base_heap (ghost_ref a pcm) emp (fun r -> ghost_pts_to r x)
 
 val ghost_read
-    (#ex:inames base_heap)
-    (#meta:erased bool)
     (#a:Type)
     (#p:pcm a)
     (r:ghost_ref a p)
@@ -165,68 +128,47 @@ val ghost_read
     (f:(v:a{compatible p x v}
         -> GTot (y:a{compatible p y v /\
                      FStar.PCM.frame_compatible p x v y})))
-: act:ghost_action_except base_heap (erased (v:a{compatible p x v /\ p.refine v})) ex
-        (ghost_pts_to meta r x)
-        (fun v -> ghost_pts_to meta r (f v)) {
-            preserves_inames act
-        }
+: ghost_action_except base_heap (erased (v:a{compatible p x v /\ p.refine v}))
+        (ghost_pts_to r x)
+        (fun v -> ghost_pts_to r (f v)) 
 
 val ghost_write
-    (#ex:inames base_heap)
-    (#meta:erased bool)
     (#a:Type)
     (#p:pcm a)
     (r:ghost_ref a p)
     (x y:Ghost.erased a)
     (f:FStar.PCM.frame_preserving_upd p x y)
-: act:ghost_action_except base_heap unit ex
-        (ghost_pts_to meta r x)
-        (fun _ -> ghost_pts_to meta r y) {
-            reveal meta == false ==> preserves_inames act
-        }
+: ghost_action_except base_heap unit
+        (ghost_pts_to r x)
+        (fun _ -> ghost_pts_to r y)
 
 val ghost_share
-    (#ex:inames base_heap)
-    (#meta:erased bool)
     (#a:Type)
     (#pcm:pcm a)
     (r:ghost_ref a pcm)
     (v0:FStar.Ghost.erased a)
     (v1:FStar.Ghost.erased a{composable pcm v0 v1})
-: act:ghost_action_except base_heap unit ex
-    (ghost_pts_to meta r (v0 `op pcm` v1))
-    (fun _ -> ghost_pts_to meta r v0 `base_heap.star` ghost_pts_to meta r v1) {
-        preserves_inames act
-    }
-
+: ghost_action_except base_heap unit
+    (ghost_pts_to r (v0 `op pcm` v1))
+    (fun _ -> ghost_pts_to r v0 `base_heap.star` ghost_pts_to r v1)
 
 val ghost_gather
-    (#ex:inames base_heap)
-    (#meta:erased bool)
     (#a:Type)
     (#pcm:pcm a)
     (r:ghost_ref a pcm)
     (v0:FStar.Ghost.erased a)
     (v1:FStar.Ghost.erased a)
-: act:ghost_action_except base_heap (squash (composable pcm v0 v1)) ex
-    (ghost_pts_to meta r v0 `base_heap.star` ghost_pts_to meta r v1)
-    (fun _ -> ghost_pts_to meta r (op pcm v0 v1)) {
-        preserves_inames act
-    }
+: ghost_action_except base_heap (squash (composable pcm v0 v1))
+    (ghost_pts_to r v0 `base_heap.star` ghost_pts_to r v1)
+    (fun _ -> ghost_pts_to r (op pcm v0 v1))
 
 val extend
-    (#ex:inames base_heap)
-    (#a:Type u#a)
+    (#a:Type)
     (#pcm:pcm a)
     (x:a{pcm.refine x})
-: act:action_except base_heap (ref a pcm) ex    
-        base_heap.emp 
-        (fun r -> pts_to r x) {
-            preserves_inames act
-        }
+: action_except base_heap (ref a pcm) emp (fun r -> pts_to r x)
 
 val read
-    (#ex:inames base_heap)
     (#a:Type)
     (#p:pcm a)
     (r:ref a p)
@@ -234,67 +176,154 @@ val read
     (f:(v:a{compatible p x v}
         -> GTot (y:a{compatible p y v /\
                      FStar.PCM.frame_compatible p x v y})))
-: act:action_except base_heap (v:a{compatible p x v /\ p.refine v}) ex
+: action_except base_heap (v:a{compatible p x v /\ p.refine v})
     (pts_to r x)
-    (fun v -> pts_to r (f v)) {
-        preserves_inames act
-    }
+    (fun v -> pts_to r (f v))
 
 val write
-    (#ex:inames base_heap)
     (#a:Type)
     (#p:pcm a)
     (r:ref a p)
     (x y:Ghost.erased a)
     (f:FStar.PCM.frame_preserving_upd p x y)
-: act:action_except base_heap unit ex
+: action_except base_heap unit
     (pts_to r x)
-    (fun _ -> pts_to r y) {
-        preserves_inames act
-    }
+    (fun _ -> pts_to r y)
 
 val share
-    (#ex:inames base_heap)
     (#a:Type)
     (#pcm:pcm a)
     (r:ref a pcm)
     (v0:FStar.Ghost.erased a)
     (v1:FStar.Ghost.erased a{composable pcm v0 v1})
-: act:ghost_action_except base_heap unit ex
+: ghost_action_except base_heap unit
     (pts_to r (v0 `op pcm` v1))
-    (fun _ -> pts_to r v0 `base_heap.star` pts_to r v1) {
-        preserves_inames act
-    }
+    (fun _ -> pts_to r v0 `base_heap.star` pts_to r v1)
 
 val gather
-    (#ex:inames base_heap)
     (#a:Type)
     (#pcm:pcm a)
     (r:ref a pcm)
     (v0:FStar.Ghost.erased a)
     (v1:FStar.Ghost.erased a)
-: act:ghost_action_except base_heap (squash (composable pcm v0 v1)) ex
+: ghost_action_except base_heap (squash (composable pcm v0 v1))
     (pts_to r v0 `base_heap.star` pts_to r v1)
-    (fun _ -> pts_to r (op pcm v0 v1)) {
-        preserves_inames act
-    }
+    (fun _ -> pts_to r (op pcm v0 v1))
 
 val pts_to_not_null_action 
-      (#ex:inames base_heap)
       (#a:Type u#a)
       (#pcm:pcm a)
       (r:erased (ref a pcm))
       (v:Ghost.erased a)
-: act:ghost_action_except base_heap (squash (not (is_null r))) ex
+: ghost_action_except base_heap (squash (not (is_null r)))
     (pts_to r v)
-    (fun _ -> pts_to r v) {
-        preserves_inames act
-    }
+    (fun _ -> pts_to r v)
 
-val exists_congruence 
-        (#a:Type u#a)
-        (w:a)
-        (p:a -> base_heap.slprop)
-: Lemma 
-    (requires forall x. is_boxable (p x))
-    (ensures is_boxable (exists_ p))
+val ghost_pts_to' (#a:Type u#a) (#p:pcm a) (r:ghost_ref a p) (x:a) : (base_heap u#(max a b)).slprop
+
+val ghost_extend'
+    (#a:Type u#a)
+    (#pcm:pcm a)
+    (x:erased a{pcm.refine x})
+: ghost_action_except base_heap (ghost_ref a pcm) emp (fun r -> ghost_pts_to' u#a u#b r x)
+
+val ghost_read'
+    (#a:Type)
+    (#p:pcm a)
+    (r:ghost_ref a p)
+    (x:erased a)
+    (f:(v:a{compatible p x v}
+        -> GTot (y:a{compatible p y v /\
+                     FStar.PCM.frame_compatible p x v y})))
+: ghost_action_except base_heap (erased (v:a{compatible p x v /\ p.refine v}))
+        (ghost_pts_to' u#a u#b r x)
+        (fun v -> ghost_pts_to' u#a u#b r (f v)) 
+
+val ghost_write'
+    (#a:Type)
+    (#p:pcm a)
+    (r:ghost_ref a p)
+    (x y:Ghost.erased a)
+    (f:FStar.PCM.frame_preserving_upd p x y)
+: ghost_action_except base_heap unit
+        (ghost_pts_to' u#a u#b r x)
+        (fun _ -> ghost_pts_to' u#a u#b r y)
+
+val ghost_share'
+    (#a:Type)
+    (#pcm:pcm a)
+    (r:ghost_ref a pcm)
+    (v0:FStar.Ghost.erased a)
+    (v1:FStar.Ghost.erased a{composable pcm v0 v1})
+: ghost_action_except base_heap unit
+    (ghost_pts_to' u#a u#b r (v0 `op pcm` v1))
+    (fun _ -> ghost_pts_to' u#a u#b r v0 `base_heap.star` ghost_pts_to' u#a u#b r v1)
+
+val ghost_gather'
+    (#a:Type)
+    (#pcm:pcm a)
+    (r:ghost_ref a pcm)
+    (v0:FStar.Ghost.erased a)
+    (v1:FStar.Ghost.erased a)
+: ghost_action_except base_heap (squash (composable pcm v0 v1))
+    (ghost_pts_to' u#a u#b r v0 `base_heap.star` ghost_pts_to' u#a u#b r v1)
+    (fun _ -> ghost_pts_to' u#a u#b r (op pcm v0 v1))
+
+val pts_to' (#a:Type u#a) (#p:pcm a) (r:ref a p) (x:a) : (base_heap u#(max a b)).slprop
+
+val extend'
+    (#a:Type)
+    (#pcm:pcm a)
+    (x:a{pcm.refine x})
+: action_except base_heap (ref a pcm) emp (fun r -> pts_to' u#a u#b r x)
+
+val read'
+    (#a:Type)
+    (#p:pcm a)
+    (r:ref a p)
+    (x:erased a)
+    (f:(v:a{compatible p x v}
+        -> GTot (y:a{compatible p y v /\
+                     FStar.PCM.frame_compatible p x v y})))
+: action_except base_heap (v:a{compatible p x v /\ p.refine v})
+    (pts_to' u#a u#b r x)
+    (fun v -> pts_to' u#a u#b r (f v))
+
+val write'
+    (#a:Type)
+    (#p:pcm a)
+    (r:ref a p)
+    (x y:Ghost.erased a)
+    (f:FStar.PCM.frame_preserving_upd p x y)
+: action_except base_heap unit
+    (pts_to' u#a u#b r x)
+    (fun _ -> pts_to' u#a u#b r y)
+
+val share'
+    (#a:Type)
+    (#pcm:pcm a)
+    (r:ref a pcm)
+    (v0:FStar.Ghost.erased a)
+    (v1:FStar.Ghost.erased a{composable pcm v0 v1})
+: ghost_action_except base_heap unit
+    (pts_to' u#a u#b r (v0 `op pcm` v1))
+    (fun _ -> pts_to' u#a u#b r v0 `base_heap.star` pts_to' u#a u#b r v1)
+
+val gather'
+    (#a:Type)
+    (#pcm:pcm a)
+    (r:ref a pcm)
+    (v0:FStar.Ghost.erased a)
+    (v1:FStar.Ghost.erased a)
+: ghost_action_except base_heap (squash (composable pcm v0 v1))
+    (pts_to' u#a u#b r v0 `base_heap.star` pts_to' u#a u#b r v1)
+    (fun _ -> pts_to' u#a u#b r (op pcm v0 v1))
+
+val pts_to_not_null_action'
+      (#a:Type u#a)
+      (#pcm:pcm a)
+      (r:erased (ref a pcm))
+      (v:Ghost.erased a)
+: ghost_action_except base_heap (squash (not (is_null r)))
+    (pts_to' u#a u#b r v)
+    (fun _ -> pts_to' u#a u#b r v)
