pulse/lib/core/PulseCore.HeapSig.fsti
@@ -99,14 +99,6 @@ type heap_sig : Type u#(a + 2) = {
     );
     non_info_slprop: non_info slprop;
 
-    bprop : Type u#a;
-    up: bprop -> slprop;
-    down: slprop -> bprop;
-    up_down: (
-      p:bprop ->
-      Lemma (down (up p) == p)
-    );
-
     emp : slprop;
     pure : prop -> slprop;
     star : slprop -> slprop -> slprop;
@@ -127,17 +119,6 @@ type heap_sig : Type u#(a + 2) = {
       p:slprop ->
       Lemma (p == (p `star` emp))
     );
-    // star_commutative: (
-    //   p:slprop ->
-    //   q:slprop ->
-    //   Lemma (p `star` q == q `star` p)
-    // );
-    // star_associative: (
-    //   p:slprop ->
-    //   q:slprop ->
-    //   r:slprop ->
-    //   Lemma (p `star` (q `star` r) == (p `star` q) `star` r)
-    // );
     star_equiv: (
       p:slprop ->
       q:slprop ->
@@ -150,97 +131,15 @@ type heap_sig : Type u#(a + 2) = {
           interp p m0 /\
           interp q m1))
     );
-    star_congruence: (
-      p:slprop ->
-      q:slprop ->
-      Lemma 
-      (requires up (down p) == p /\ up (down q) == q)
-      (ensures up (down (p `star` q)) == p `star` q)
-    );
-    // pts_to: (
-    //   #a:Type u#a ->
-    //   #p:pcm a ->
-    //   ref a p ->
-    //   a ->
-    //   slprop
-    // );
-
-    // ghost_pts_to: (
-    //   meta:bool ->
-    //   #a:Type u#a ->
-    //   #p:pcm a ->
-    //   ghost_ref a p ->
-    //   a ->
-    //   slprop
-    // );
-
-    iref:Type0;
-    deq_iref:FStar.GhostSet.decide_eq iref;
-    non_info_iref: non_info iref;
-    inv : iref -> slprop -> slprop;
-    iname_ok: iref -> mem -> prop;
-    dup_inv_equiv : (
-      i:iref ->
-      p:slprop ->
-      Lemma (inv i p == (inv i p `star` inv i p))
-    );
-    mem_invariant : Set.set iref -> mem -> slprop;
-    inv_iname_ok : (
-      i:iref ->
-      p:slprop ->
-      m:mem ->
-      Lemma 
-        (requires interp (inv i p) m)
-        (ensures iname_ok i m)
-    );
-    mem_invariant_equiv : (
-      e:Set.set iref ->
-      m:mem ->
-      i:iref ->
-      p:slprop ->
-      Lemma 
-        (requires
-          interp (inv i p) m /\
-          ~(i `Set.mem` e))
-        (ensures
-          mem_invariant e m ==
-          mem_invariant (add deq_iref i e) m `star` p)
-    );
-    iref_injective: (iref -> GTot bool);
-    iref_injectivity : (
-      i:iref ->
-      j:iref ->
-      p:slprop ->
-      q:slprop ->
-      m:mem ->
-      Lemma
-       (requires
-          iref_injective i /\
-          iref_injective j /\
-          interp (inv i p) m /\
-          interp (inv j q) m)
-       (ensures
-         (p =!= q ==> i =!= j) /\
-         (i==j ==> p == q))
-    );
-    empty_mem_invariant : (e:Set.set iref -> Lemma (mem_invariant e sep.empty == emp))
 }
 
 val star_commutative (#h: heap_sig) (p q: h.slprop) : Lemma (p `h.star` q == q `h.star` p)
 val star_associative (#h: heap_sig) (p q r: h.slprop) : Lemma (p `h.star` (q `h.star` r) == (p `h.star` q) `h.star` r)
 
-let add_iref (#h:heap_sig) (i:h.iref) (s:GhostSet.set h.iref) = add h.deq_iref i s
 val emp_trivial (h:heap_sig u#a)
 : Lemma (forall m. h.interp h.emp m)
 
-let is_boxable (#h:heap_sig u#a) (p:h.slprop) : prop = h.up (h.down p) == p 
-let boxable (h:heap_sig u#a) = p:h.slprop { is_boxable p }
-
 let interpret (#h:heap_sig u#h) (p:h.slprop) : h.mem -> prop = fun m -> h.interp p m
-let inames (hs:heap_sig u#h) = Set.set hs.iref
-let inames_ok (#hs:heap_sig u#h) (is:inames hs) (m:hs.mem)
-: prop
-= forall (i:hs.iref). i `Set.mem` is ==> hs.iname_ok i m
 let full_mem (hs:heap_sig u#h) = m:hs.mem{ hs.full_mem_pred m }
 let maybe_ghost_action (chs:heap_sig u#m) (maybe_ghost:bool) (m0 m1:chs.mem)
     = maybe_ghost ==> chs.is_ghost_action m0 m1
@@ -249,47 +148,41 @@ let step_t
   (chs:heap_sig u#m)
   (a:Type u#a)
   (maybe_ghost:bool)
-  (except:inames chs)
   (expects:chs.slprop)
   (provides: a -> GTot chs.slprop)
   (frame:chs.slprop)
 = ST.st #(full_mem chs) a
     (requires fun m0 ->
-        inames_ok except m0 /\
-        interpret (expects `chs.star` frame `chs.star` chs.mem_invariant except m0) m0)
+        interpret (expects `chs.star` frame) m0)
     (ensures fun m0 x m1 ->
         maybe_ghost_action chs maybe_ghost m0 m1 /\
-        inames_ok except m1 /\
-        interpret (expects `chs.star` frame `chs.star` chs.mem_invariant except m0) m0 /\  //TODO: fix the effect so as not to repeat this
-        interpret (provides x `chs.star` frame `chs.star` chs.mem_invariant except m1) m1)
+        interpret (expects `chs.star` frame) m0 /\  //TODO: fix the effect so as not to repeat this
+        interpret (provides x `chs.star` frame) m1)
 
 (** An action is just a thunked computation in [MstTot] that takes a frame as argument *)
 let _action_except 
     (chs:heap_sig u#m)
     (a:Type u#a)
     (maybe_ghost:bool)
-    (except:inames chs)
     (expects:chs.slprop)
     (provides: a -> GTot chs.slprop)
  : Type u#(max a (m + 1)) 
- = frame:chs.slprop -> step_t chs a maybe_ghost except expects provides frame
+ = frame:chs.slprop -> step_t chs a maybe_ghost expects provides frame
 
 #push-options "--print_universes --print_implicits"
 let action_except
     (chs:heap_sig u#m)
     (a:Type u#a)
-    (except:inames chs)
     (expects:chs.slprop)
     (provides:a -> GTot chs.slprop)
-= _action_except chs a false except expects provides
+= _action_except chs a false expects provides
 
 let ghost_action_except
       (chs:heap_sig u#m)
       (a:Type u#a)
-      (except:inames chs)
       (expects:chs.slprop)
       (provides: a -> GTot chs.slprop)
-= _action_except chs a true except expects provides
+= _action_except chs a true expects provides
 
 val exists_
     (#chs:heap_sig u#m)
@@ -328,33 +221,13 @@ val ac_lemmas (h:heap_sig u#a)
 
 val frame
       (#h:heap_sig u#h)
-      (#opened_invariants:inames h)
       (#maybe_ghost:bool)
       (#a:Type u#a)
       (#pre:h.slprop)
       (#post:a -> GTot h.slprop)
       (frame:h.slprop)
-      ($f:_action_except h a maybe_ghost opened_invariants pre post)
-: _action_except h a maybe_ghost opened_invariants (pre `h.star` frame) (fun x -> post x `h.star` frame)
-
-val witness_exists 
-      (#h:heap_sig u#h)
-      (#opened_invariants:inames h)
-      (#a:Type u#a)
-      (p:a -> GTot h.slprop)
-: ghost_action_except h (erased a) opened_invariants
-           (exists_ p)
-           (fun x -> p x)
-
-val intro_exists
-      (#h:heap_sig u#h)
-      (#opened_invariants:_)
-      (#a:Type u#a)
-      (p:a -> GTot h.slprop)
-      (x:erased a)
-: ghost_action_except h unit opened_invariants
-      (p x)
-      (fun _ -> exists_ p)
+      ($f:_action_except h a maybe_ghost pre post)
+: _action_except h a maybe_ghost (pre `h.star` frame) (fun x -> post x `h.star` frame)
 
 module U = FStar.Universe
 let lift_dom_ghost #a #b (q:a -> GTot b) : U.raise_t a -> GTot b =
@@ -362,41 +235,36 @@ let lift_dom_ghost #a #b (q:a -> GTot b) : U.raise_t a -> GTot b =
 
 val lift_h_exists
       (#h:heap_sig u#h)
-      (#opened_invariants:_)
       (#a:Type u#a)
       (p:a -> GTot h.slprop)
-: ghost_action_except h unit opened_invariants
+: ghost_action_except h unit
     (exists_ p)
     (fun _a -> exists_ #_ #(U.raise_t a) (lift_dom_ghost p))
 
 val elim_pure
       (#h:heap_sig u#h)
-      (#opened_invariants:_)
       (p:prop)
-: ghost_action_except h (squash p) opened_invariants (h.pure p) (fun _ -> h.emp)
+: ghost_action_except h (squash p) (h.pure p) (fun _ -> h.emp)
 
 val intro_pure
       (#h:heap_sig u#h)
-      (#opened_invariants:_)
       (p:prop)
       (_:squash p)
-: ghost_action_except h unit opened_invariants h.emp (fun _ -> h.pure p)
+: ghost_action_except h unit h.emp (fun _ -> h.pure p)
   
 val drop 
       (#h:heap_sig u#h)
-      (#opened_invariants:_)
       (p:h.slprop)
-: ghost_action_except h unit opened_invariants p (fun _ -> h.emp)
+: ghost_action_except h unit p (fun _ -> h.emp)
 
 val lift_ghost
       (#h:heap_sig u#h)
-      (#opened_invariants:inames h)
       (#a:Type u#a)
       (#p:h.slprop)
       (#q:a -> GTot h.slprop)
       (ni_a:non_info a)
-      (f:erased (ghost_action_except h a opened_invariants p q))
-: ghost_action_except h a opened_invariants p q
+      (f:erased (ghost_action_except h a p q))
+: ghost_action_except h a p q
 
 val destruct_star (#h:heap_sig u#h) (p q:h.slprop) (m:h.mem)
 : Lemma (h.interp (p `h.star` q) m ==> h.interp p m /\ h.interp q m)
@@ -405,5 +273,3 @@ val intro_pure_frame (#h:heap_sig u#h) (p:h.slprop) (q:prop) (_:squash q) (m:h.m
 : Lemma
   (requires h.interp p m)
   (ensures h.interp (p `h.star` h.pure q) m)
-
-let is_storable (#h:heap_sig) (p:h.slprop) = h.up (h.down p) == p
